libs/ffi/mitlsffi.h
@@ -122,12 +122,20 @@ typedef struct {
   size_t len;
   char ticket[MAX_TICKET_LEN];
 } quic_ticket;
-  
+
+// This length is somehow arbitrary
+#define MAX_OTHERS_LEN 1024 
+
 typedef struct {
   unsigned int max_stream_data;
   unsigned int max_data;
   unsigned int max_stream_id;
   unsigned short idle_timeout;
+
+  // The custom parameters are still in RFC wire format:
+  // a sequence of (descriptor: 2; len: 2; data: len) bytes
+  size_t others_len;
+  char others[MAX_OTHERS_LEN]; 
 } quic_transport_parameters;
 
 typedef struct quic_key quic_key;
@@ -160,7 +168,7 @@ extern int MITLS_CALLCONV FFI_mitls_quic_create(/* out */ quic_state **state, qu
 
 extern quic_result MITLS_CALLCONV FFI_mitls_quic_process(/* in */ quic_state *state, /*in*/ char* inBuf, /*inout*/ size_t *pInBufLen, /*out*/ char *outBuf, /*inout*/ size_t *pOutBufLen, /* out */ char **errmsg);
 
-extern int MITLS_CALLCONV FFI_mitls_quic_get_transport_parameters(/* in */ quic_state *state, /*out*/ quic_transport_parameters *qp);
+extern int MITLS_CALLCONV FFI_mitls_quic_get_peer_parameters(/* in */ quic_state *state, /*out*/ quic_transport_parameters *qp, /* out */ char **errmsg);
 extern int MITLS_CALLCONV FFI_mitls_quic_get_exporter(/* in */ quic_state *state, int early, /* out */ quic_secret *secret, char **errmsg);
 extern int MITLS_CALLCONV FFI_mitls_quic_get_ticket(/* in */ quic_state *state, /*out*/ quic_ticket *ticket , /* out */ char **errmsg);
 extern void MITLS_CALLCONV FFI_mitls_quic_free(/* in */ quic_state *state);
